Defined nominal induction; WIP proof of weakening

Stlc/nomstlc.v
@@ -44,10 +44,10 @@ Notation "A :-> B" := (tArr A B) (at level 70).
 
 (** The syntax for STLC. We use [Atom] type to represent variable names *)
 Inductive Exp : Type :=
-  | Int : Atom -> Exp
-  | Var : Atom -> Exp
-  | Lam : Atom -> Exp -> Exp
-  | App : Exp -> Exp -> Exp.
+  | Int (n : nat)
+  | Var (a : Atom)
+  | Lam (a : Atom) (e : Exp)
+  | App (e1 : Exp) (e2 : Exp).
 
 (** Action of a permutation [p] on epressions [Exp] *)
 Fixpoint ac_exp (p : Perm) (e : Exp) : Exp :=
@@ -63,7 +63,7 @@ Fixpoint supp_exp (e : Exp) : Atom.V.t :=
   match e with
   | Int n => empty
   | Var v => singleton v
-  | Lam v e1 => add v (supp_exp e1)
+  | Lam v e1 => union (singleton v) (supp_exp e1)
   | App e1 e2 => union (supp_exp e1) (supp_exp e2)
   end.
 
@@ -101,7 +101,7 @@ Instance NomExp : NomSet.
   + simpl. rewrite H;auto with set.
   + simpl. rewrite H;simpl;auto with set.
     rewrite IHe;auto.
-    intros a Ha. apply H. simpl;auto with set.
+    intros a0 Ha. apply H. simpl;auto with set.
   + simpl.
     assert (He1 : forall a, In a (supp_exp e1) -> perm p a = a) by
         (intros;apply H;simpl;auto with set).
@@ -129,9 +129,11 @@ Inductive ae_exp : NomExp -> NomExp -> Prop :=
     (Int n) =α (Int n)
 | ae_var : forall (a : NomAtom),
     (Var a) =α (Var a)
-| ae_lam : forall (a b c : NomAtom) (e1 e2 : NomExp),
-    c ## (a, b, vars_exp e1, vars_exp e2) ->
-    ((swap a c) @ e1) =α ((swap b c) @ e2) ->
+| ae_lam : forall (a b : NomAtom) (e1 e2 : NomExp) (vs : PFin),
+    (* this is equivalent to explicitly specifying [c ## (a, b, vars_exp e1, vars_exp e2])
+    see "Alpha-Structural Induction and Recursion for the Lambda Calculus in Constructive Type Theory"*)
+    (forall (c : NomAtom), c # vs ->
+    ((swap a c) @ e1) =α ((swap b c) @ e2)) ->
     (Lam a e1) =α (Lam b e2)
 | ae_app : forall e1 e2 e1' e2',
     e1 =α e1' ->
@@ -201,28 +203,9 @@ Example identity_alpha_equiv :
   forall x y, (Lam x (Var x)) =α (Lam y (Var y)).
 Proof.
   intros x y.
-  destruct (Atom.Atom_inf (union (singleton x) (singleton y))) as [z Hz].
-  assert (Hneq : z <> x /\ z <> y) by
-      (split; unfold not; intros; apply Hz; auto with set).
-  apply ae_lam with (c:=z); repeat split;
-    try (simpl; unfold fresh; rewrite Disjoint_spec; intros u;
-         unfold not; intros; apply Hz; simpl in *; repeat rewrite singleton_spec in *).
-  - assert (z = x) by (destruct H; congruence).
-    subst. intuition;tryfalse.
-  - assert (z = y) by (destruct H; congruence).
-    subst. intuition;tryfalse.
-  - assert (z = x) by (destruct H; simpl in *;  congruence).
-    subst. intuition;tryfalse.
-  - assert (z = y) by (destruct H; simpl in *;  congruence).
-    subst. intuition;tryfalse.
-  - simpl. unfold swap_fn.
-    destruct Hneq as [L R].
-    assert (H : SetProperties.P.FM.eq_dec z x = right L) by apply eq_dec_neq'.
-    rewrite H.
-    assert (H' : SetProperties.P.FM.eq_dec z y = right R) by apply eq_dec_neq'.
-    rewrite H'.
-    repeat rewrite eq_dec_refl.
-    constructor.
+  apply ae_lam with (vs:=empty).
+  intros. simpl. unfold swap_fn.
+  now repeat rewrite eq_dec_refl.
 Qed.
 
 (** ** Typing *)
@@ -250,7 +233,7 @@ Fixpoint ac_env {A : Type} (p : Perm) (e : Env (A:=A)) :=
 Fixpoint dom {A : Type} (env : Env (A:=A)) : PFin :=
   match env with
   | empty => Atom.V.empty
-  | cons env1 a e => add a (dom env1)
+  | cons env1 a e => (singleton a) ∪ (dom env1)
   end.
 
 (** Nominal set of environments*)
@@ -342,19 +325,19 @@ Proof.
     apply set_extensionality.
     intros e'. split.
     + intros. rewrite set_map_iff in *. 
-      rewrite TSetMod.OP.P.Dec.F.add_iff in *.
+      rewrite TSetMod.OP.P.Dec.F.union_iff in *.
       rewrite set_map_iff in *.
       destruct H as [Heq|Htl].
-      * exists c. split;intuition;auto with set.
+      * exists c. split;try symmetry;auto with set.
       * destruct Htl as [e'' He''].
         exists e'';intuition;eauto with set.
     + intros. rewrite set_map_iff in *. 
-      rewrite TSetMod.OP.P.Dec.F.add_iff in *.
+      rewrite TSetMod.OP.P.Dec.F.union_iff in *.
       rewrite set_map_iff in *.
       destruct H as [e'' He'']. destruct He'' as [L R].
-      rewrite TSetMod.OP.P.Dec.F.add_iff in *.
+      rewrite TSetMod.OP.P.Dec.F.union_iff in *.
       destruct R.
-      * left;subst;congruence.
+      * left;subst. auto with set.
       * right. exists e''.
       subst. split;auto.
 Qed.
@@ -405,3 +388,507 @@ Proof.
   intros x y p Hty.
   induction Hty;econstructor;eauto.
 Qed.
+
+Lemma equivar_Typing_inv ty :
+  forall (x : NomEnv) (y : NomExp) (p : Perm),
+   [p @ x |- p @ y ::: ty] -> [x |- y ::: ty].
+Proof.
+  intros.
+  (* specialize (equivar_Typing ty _ _ (- p) H) as HH. with (p:=perm_inv p) in H. *)
+  (* unfold equivar_rel. *)
+Admitted.
+
+Lemma fresh_atom_neq_iff (a b : NomAtom) : a # b <-> a <> b.
+Proof.
+  split.
+  + intros Hab. unfold fresh in *.
+    rewrite TSetMod.Disjoint_spec in Hab;intuition; eauto with set.
+  + intros H.
+    unfold fresh in *.
+    rewrite TSetMod.Disjoint_spec in *. intros ? H0.
+    destruct H0.
+    assert (a = k /\ b = k) by auto with set.
+    intuition;tryfalse.
+Qed.
+
+Lemma fresh_atom_singleton (a b : NomAtom) : a # (singleton b : PFin) <-> a # b.
+Proof.
+  split;intros;eauto with set.
+Qed.
+
+
+Hint Resolve fresh_atom_singleton : set.
+Hint Resolve <- fresh_atom_neq_iff : set.
+Hint Resolve -> fresh_atom_neq_iff : set.
+
+Lemma swap_compose_neq (a b c z : NomAtom) :
+  b # z ->
+  c # z ->
+  (((swap b c ∘p swap a b) z) = ((swap a c) z)).
+Proof.
+  unfold swap, swap_fn, fresh;cbn.
+  intros Hb Hc.
+  assert (Hc_neq : c <> z) by auto with set.
+  assert (b <> z) by auto with set.
+  cbn in *. unfold fresh, swap_fn in *.
+  destruct (eq_dec a z);
+    destruct (eq_dec b z);subst;try rewrite eq_dec_refl;auto.
+  destruct (eq_dec z a);tryfalse.
+  destruct (eq_dec b z);tryfalse.
+  destruct (eq_dec c z);tryfalse.
+  reflexivity.
+Qed.
+  
+Lemma swap_action_compose_fresh (a b c : NomAtom) (e : NomExp) :
+  b # (supp e : PFin) ->
+  c # (supp e : PFin) ->
+  (((swap b c ∘p swap a b) @ e) = ((swap a c) @ e)).
+Proof.
+  intros Hb Hc.
+  induction e;auto.
+  + unfold swap_fn.
+    assert (Hc_neq : c <> a0) by auto with set.
+    assert (b <> a0) by auto with set.
+    cbn. apply f_equal.
+    now apply swap_compose_neq.
+  + cbn in *. rewrite fresh_union_iff in *.
+    assert (Hc_fresh : (c : NomAtom) # (a0 : NomAtom)) by (intuition;auto with set).
+    assert (Hc_neq : c <> a0) by (destruct Hb;auto with set).
+    assert (Hb_fresh : (c : NomAtom) # (a0 : NomAtom)) by (destruct Hb; auto with set).
+    assert (Hb_neq : b <> a0) by (destruct Hb;auto with set).
+    rewrite IHe;intuition;auto.
+    apply f_equal2.
+    * now apply swap_compose_neq.
+    * reflexivity.
+  + cbn in *.
+    rewrite fresh_union_iff in *.
+    apply f_equal2;intuition;auto.
+Qed.
+
+Lemma Exp_perm_ind (P : Exp -> Prop)
+      (Hint : forall n : nat, P (Int n))
+      (Hvar : forall a : Atom, P (Var a))
+      (Hlam : forall (a : Atom) (e : Exp), (forall (π : Perm), P (π @ e)) -> P (Lam a e))
+      (Happ : forall e : Exp, P e -> forall e0 : Exp, P e0 -> P (App e e0)) :
+      forall e : Exp, P e.
+Proof.
+  intros e.
+  assert (H : forall π, P (π @ e)).
+  {induction e;intros;cbn;auto.
+   cbn. apply Hlam with (a:=π a)(e:= @action NomExp π e).
+   intros;rewrite action_compose. apply IHe. }
+  rewrite <- (action_id (NomSet:=NomExp)).
+  apply H.
+Qed.
+
+Lemma Exp_perm_rect (P : Exp -> Type)
+      (Hint : forall n : nat, P (Int n))
+      (Hvar : forall a : Atom, P (Var a))
+      (Hlam : forall (a : Atom) (e : Exp), (forall (π : Perm), P (π @ e)) -> P (Lam a e))
+      (Happ : forall e : Exp, P e -> forall e0 : Exp, P e0 -> P (App e e0)) :
+      forall e : Exp, P e.
+Proof.
+  intros e.
+  assert (H : forall π, P (π @ e)).
+  {induction e;intros;cbn;auto.
+   cbn. apply Hlam with (a:=π a)(e:= @action NomExp π e).
+   intros;rewrite action_compose. apply IHe. }
+  rewrite <- (action_id (NomSet:=NomExp)).
+  apply H.
+Defined.
+
+Definition Exp_perm_rect' (P : Exp -> Type)
+      (Hint : forall n : nat, P (Int n))
+      (Hvar : forall a : Atom, P (Var a))
+      (Hlam : forall (a : Atom) (e : Exp), (forall (π : Perm), P (π @ e)) -> P (Lam a e))
+      (Happ : forall e : Exp, P e -> forall e0 : Exp, P e0 -> P (App e e0)) :
+      forall (e : Exp) (π : Perm), P (π @ e).
+  refine (fix go e := _).
+  destruct e.
+  - intros;apply Hint.
+  - intros;apply Hvar.
+  - intros π. cbn. apply Hlam with (a:=π a)(e:= @action NomExp π e).
+    intros π0;rewrite action_compose. apply go.
+  - intros π. apply Happ; fold ac_exp; apply go.
+Defined.
+
+Definition Exp_perm_rec {A}
+           (Hint : nat -> A)
+           (Hvar : Atom -> A)
+           (Hlam : Atom -> Exp -> (Perm -> A) -> A)
+           (Happ : Exp -> A -> Exp -> A -> A) : Exp -> Perm -> A :=
+  Exp_perm_rect' (fun _ => A) Hint Hvar Hlam Happ.
+  
+
+Definition α_compatible (P : Exp -> Prop) : Prop
+  := forall e1 e2, e1 =α e2 -> P e1 -> P e2.
+
+Definition α_compatible_type (P : Exp -> Type) : Type
+  := forall e1 e2, e1 =α e2 -> P e1 -> P e2.
+
+
+Lemma ae_exp_equivariant :
+  equivar_rel ae_exp.
+Proof.
+  intros e1 e2 π Hα.
+  revert dependent π.
+  induction Hα;intros π.
+  + constructor.
+  + constructor.
+  + cbn. eapply ae_lam with (vs:= vs).
+    intros. change (ac_exp π e1) with (π @ e1).
+    rewrite action_compose.
+Admitted.
+
+Lemma ae_exp_refl (e : Exp) : e =α e.
+Proof.
+  induction e;try constructor;auto.
+  apply ae_lam with (vs:=supp (e : NomExp)).
+  intros.
+  now apply ae_exp_equivariant.
+Qed.
+
+Lemma ae_exp_sym (e1 e2 : Exp) :
+  e1 =α e2 ->
+  e2 =α e1.
+Proof.
+  Admitted.
+
+Lemma ae_exp_trans (e1 e2 e3 : Exp) :
+  e1 =α e2 ->
+  e2 =α e3 ->
+  e1 =α e3.
+Proof.
+  Admitted.
+
+(** ** An induction principle for α-compatible properties *)
+(** In the [Lam] case, we use co-finite quantification: [P (Lam a a)] holds for all [a] apart from a finite set of variables [vs] *)
+Lemma Exp_alpha_equiv_ind :
+  forall P : Exp -> Prop,
+    α_compatible P ->
+    (forall n : nat, P (Int n)) ->
+    (forall (a : NomAtom), P (Var a)) ->
+    (exists (vs : PFin), forall (a : NomAtom),
+          a # vs -> forall (e : Exp), P e -> P (Lam a e)) ->
+    (forall e : Exp, P e -> forall e0 : Exp, P e0 -> P (App e e0)) ->
+    forall e : Exp, P e.
+Proof.
+  intros ? Hα Hint Hvar Hlam Happ e.
+  apply Exp_perm_ind;auto.
+  + intros a e0 He0.
+    destruct Hlam as [vs Hlam].
+    unfold α_compatible in Hα.
+    set (get_fresh (vs ∪ singleton a ∪ supp (e0 : NomExp))) as b.
+    cbn in *.
+    destruct b as [b fresh_b].
+    repeat rewrite fresh_union_iff in fresh_b.
+    destruct fresh_b as [[Hb_vs Hb_a] Hb_e0].
+    set ((swap a b) @ (Lam a e0 : NomExp)) as M.
+    assert (Mα : M =α Lam a e0).
+    { cbn in M.
+      eapply ae_lam with (vs:=supp (e0 : NomExp));auto.
+      unfold swap_fn. rewrite eq_dec_refl.
+      intros.
+      change ((swap b c @ ((swap a b) @ e0)) =α (swap a c @ e0)).
+      rewrite action_compose.
+      rewrite swap_action_compose_fresh;auto.
+      apply ae_exp_refl. }
+    assert (H : P ((swap a b) @ (Lam a e0))).
+      { apply Hlam.
+        + cbn. unfold swap_fn. now rewrite eq_dec_refl.
+        + apply He0. }
+      specialize (Hα _ _ Mα).
+      apply Hα. apply H.
+Qed.
+
+Lemma Exp_alpha_equiv_ind_ctx :
+  forall (P : TEnv -> Atom -> Exp -> Prop),
+    (forall ctx a, α_compatible (P ctx a)) ->
+    (forall ctx a (n : nat), P ctx a (Int n)) ->
+    (forall ctx a (a0 : NomAtom), P ctx a (Var a0)) ->
+    (forall (ctx : TEnv) a, exists (vs : PFin),  forall (a0 : NomAtom),
+        a0 # ((supp ctx ∪ vs ∪ singleton a) : PFin) ->
+        forall (e : Exp), (forall ctx0 a1, P ctx0 a1 e) -> P ctx a (Lam a0 e)) ->
+    (forall ctx a (e : Exp), P ctx a e -> forall e0 : Exp, P ctx a e0 -> P ctx a (App e e0)) ->
+    forall ctx a (e : Exp), P ctx a e.
+Proof.
+  intros P Hα Hint Hvar Hlam Happ vs a e.
+  revert a.
+  revert vs.
+  apply Exp_perm_ind with (P:=fun e => forall (ctx : TEnv) (a : Atom), P ctx a e);auto.
+  + intros a0 e0 He0 ctx a.
+    destruct (Hlam ctx a) as [vs0 Hlam'].
+    unfold α_compatible in Hα.
+    set (get_fresh (supp ctx ∪ vs0 ∪ singleton a ∪ singleton a0 ∪ supp (e0 : NomExp))) as b.
+    cbn in *.
+    destruct b as [b fresh_b].
+    repeat rewrite fresh_union_iff in fresh_b.
+    destruct fresh_b as [[[Hb_vs Hb_vs0] Hb_a] Hb_e0].
+    set ((swap a0 b) @ (Lam a0 e0 : NomExp)) as M.
+    assert (Mα : M =α Lam a0 e0).
+    { cbn in M.
+      eapply ae_lam with (vs:=supp (e0 : NomExp));auto.
+      unfold swap_fn. rewrite eq_dec_refl.
+      intros.
+      change ((swap b c @ ((swap a0 b) @ e0)) =α (swap a0 c @ e0)).
+      rewrite action_compose.
+      rewrite swap_action_compose_fresh;auto.
+      apply ae_exp_refl. }
+    assert (H : P ctx a ((swap a0 b) @ (Lam a0 e0))).
+      { apply Hlam'.
+        + cbn. unfold swap_fn. rewrite eq_dec_refl.
+          intuition;eauto with set.
+        + intros ctx0. apply He0. }
+      specialize (Hα ctx a _ _ Mα).
+      apply Hα. apply H.
+Qed.
+
+Lemma Exp_alpha_equiv_rect :
+  forall P : Exp -> Type,
+    α_compatible_type P ->
+    (forall n : nat, P (Int n)) ->
+    (forall a : NomAtom, P (Var a)) ->
+    ({vs : PFin & forall (a : NomAtom) (e : Exp),
+          a # vs -> P e -> P (Lam a e)}) ->
+    (forall e : Exp, P e -> forall e0 : Exp, P e0 -> P (App e e0)) ->
+    forall e : Exp, P e.
+Proof.
+  intros ? Hα Hint Hvar Hlam Happ e.
+  apply Exp_perm_rect;auto.
+  intros a e0 He0.
+  destruct Hlam as [vs Hlam].
+  unfold α_compatible in Hα.
+  (* set (get_fresh (vs ∪ singleton a ∪ supp (e0 : NomExp))) as b. *)
+  set (get_fresh (vs ∪ supp (e0 : NomExp))) as b.
+  cbn in *.
+  destruct b as [b fresh_b].
+  apply fresh_union_iff in fresh_b.
+  (* repeat rewrite fresh_union_iff in fresh_b. *)
+  destruct fresh_b.
+    (* as [[Hb_vs Hb_a] Hb_e0]. *)
+  set ((swap a b) @ (Lam a e0 : NomExp)) as M.
+  assert (Mα : M =α Lam a e0).
+  { cbn in M.
+    eapply ae_lam with (vs:=supp (e0 : NomExp));auto.
+    unfold swap_fn. rewrite eq_dec_refl.
+    intros.
+    change ((swap b c @ ((swap a b) @ e0)) =α (swap a c @ e0)).
+    rewrite action_compose.
+    rewrite swap_action_compose_fresh;auto.
+    apply ae_exp_refl. }
+  assert (Hswap : P ((swap a b) @ (Lam a e0))).
+    { apply Hlam.
+      + cbn. unfold swap_fn. now rewrite eq_dec_refl.
+      + fold ac_exp. apply He0. }
+    specialize (Hα _ _ Mα).
+    apply Hα. apply Hswap.
+Defined.
+
+Definition Exp_alpha_rec {A}
+           (Hint : nat -> A)
+           (Hvar : Atom -> A)
+           (Hlam : PFin * (Atom -> Exp -> A -> A))
+           (Happ : Exp -> A -> Exp -> A -> A) : Exp -> A.
+  refine (Exp_alpha_equiv_rect (fun _ => A) (fun _ _ _ => id) Hint Hvar _ Happ).
+  destruct Hlam as [vs f].
+  apply (existT _ vs).
+  intros v e ? a0. exact (f v e a0).
+Defined.
+
+Definition get_canonical : Exp -> PFin -> Exp :=
+   (Exp_alpha_rec (A:=PFin -> Exp)
+    (fun n _ => Int n)
+    (fun v _ => Var v)
+    ((Atom.V.empty, fun v body f vs => Lam v (f (singleton v ∪ vs))))
+    (fun e1 _ e2 _ _ => App e1 e2)).
+
+Example test_alpha_rec1 x :
+  get_canonical (Lam x (Var x)) Atom.V.empty = (Lam x (Var x)).
+Proof.
+  cbn.
+  set ((Atom.V.empty ∪ singleton (id x)) ∪ singleton (id x)) as rr.
+  destruct (get_fresh _).
+  destruct (fresh_union_iff _ _ ).
+  destruct a. unfold id, swap_fn.
+  rewrite eq_dec_refl.
+Abort.
+
+Example nested_lam_alpha_equiv :
+  forall x y, (Lam y (Lam x (Var x))) =α (Lam x (Lam x (Var x))).
+Proof.
+  intros x y.
+  apply ae_lam with (vs:=AtomN.V.empty).
+  intros. simpl. unfold swap_fn.
+  repeat rewrite eq_dec_refl.
+  destruct (eq_dec x y).
+  - eapply ae_lam with (vs:=AtomN.V.empty). intros. unfold swap, swap_fn;cbn.
+    now repeat rewrite eq_dec_refl.
+  - destruct (eq_dec c y).
+    * eapply ae_lam with (vs:=AtomN.V.empty). intros. unfold swap, swap_fn;cbn.
+      now repeat rewrite eq_dec_refl.
+    * eapply ae_lam with (vs:=AtomN.V.empty). intros. unfold swap, swap_fn;cbn.
+    now repeat rewrite eq_dec_refl.
+Qed.
+
+Lemma Typing_is_NOT_α_compatible (x y : NomAtom) :
+  x # y ->
+  (forall Γ τ, α_compatible (fun e => [ Γ |- e ::: τ ])) -> False.
+Proof.
+  intros Hfresh H. unfold α_compatible in H.
+  set (Lam x (Lam x (Var x))) as e1.
+  set (Lam y (Lam x (Var x))) as e2.
+  assert (typed_e2 : [empty |- e2 ::: tInt :-> (tInt :-> tInt) ]).
+  { repeat constructor; try easy.
+    unfold fresh in *. cbn. now rewrite eq_dec_refl. }
+  assert (Hα : e2 =α e1) by apply nested_lam_alpha_equiv.
+  specialize (H empty _ _ _ Hα typed_e2) as Hfalse.
+  inversion Hfalse;subst.
+  inversion H6;subst.
+  unfold fresh in *.
+  rewrite AtomN.V.Disjoint_spec in *.
+  specialize (H5 x).
+  intuition;eauto with set.
+Qed.
+
+
+(** New typing rules for the STLC, with α-equivalence for lambdas *)
+Inductive Typing_α : TEnv -> Exp -> NomTy -> Prop :=
+  | tyInt_α : forall (Gamma : TEnv) (n : Atom),
+      [ Gamma |- (Int n) ::: tInt]
+  | tyVar_α : forall (Gamma : TEnv) (x : NomAtom) (A : Ty),
+      lookEnv Gamma x = Some A ->
+      [ Gamma |- (Var x) ::: A ]
+  | tyLam_α : forall (Gamma : TEnv) (x y : NomAtom) (b1 b2 : Exp) (A B : Ty),
+      y # Gamma ->
+      (Lam x b2) =α (Lam y b1) ->
+      [ Gamma, y ::: A |- b1 ::: B ] ->
+      [ Gamma |- (Lam x b2) ::: (A :-> B)]
+  | tyApp_α : forall (Gamma : TEnv) (f a : Exp) (A B : Ty),
+      [ Gamma |- f ::: (A :-> B) ]->
+      [ Gamma |- a ::: A ] ->
+      [ Gamma |- (App f a) ::: B ]
+where "[ Gamma |- a ::: A ]" := (Typing_α Gamma a A).
+
+Lemma fresh_cons_env {A : Type} (Γ : @NomEnv A) (x y : NomAtom) (a : A):
+  x # Γ ->
+  x # y ->
+  x # ((cons Γ y a) : NomEnv).
+Proof.
+  intros Hx Hxy.
+  unfold fresh in *. cbn. rewrite Disjoint_spec in *.
+  intros ??. rewrite TSetMod.OP.P.Dec.F.union_iff in *.
+  specialize (Hx k).
+  specialize (Hxy k).
+  intuition;eauto with set.
+Qed.
+
+Example shadowing_typable x :
+  [empty |- (Lam x (Lam x (Var x))) ::: tInt :-> (tInt :-> tInt) ].
+Proof.
+  set (get_fresh (singleton x)) as c.
+  destruct c as [y Hy].
+  eapply tyLam_α with (y:=y) (b1:=(Lam x (Var x)));try easy.
+  apply ae_exp_sym.
+  apply nested_lam_alpha_equiv.
+  eapply tyLam_α with (y:=x) (b1:=(Var x)).
+  + apply fresh_cons_env;auto with set.
+    unfold fresh in *.
+    rewrite Disjoint_spec in *;intros ??.
+    specialize (Hy k). destruct H. eauto with set.
+    rewrite fresh_atom_singleton in Hy.
+    eauto with set.
+    rewrite fresh_atom_neq_iff in *.
+    now apply not_eq_sym.
+  + apply ae_exp_refl.
+  + repeat constructor. cbn. now rewrite eq_dec_refl.
+Qed.
+
+Lemma Typing_α_compatible Γ τ:
+  α_compatible (fun e => [ Γ |- e ::: τ ]).
+Proof.
+  intros e1 e2 H Hτ.
+  revert dependent e2.
+  induction Hτ;intros e2 Ha;inversion Ha;subst;clear Ha.
+  + constructor.
+  + now constructor.
+  + inversion H0;subst.
+    set (get_fresh (vs ∪ vs0 ∪ supp (e0 : NomExp) ∪ supp Gamma)) as c.
+    destruct c as [c Hc].
+    repeat rewrite fresh_union_iff in *.
+    destruct Hc as [[[Hvs Hvs0] He0] HΓ].
+    eapply tyLam_α with (y:=y) (b1:=b1);auto.
+    eapply ae_lam with (vs:=vs ∪ vs0).
+    intros.
+    repeat rewrite fresh_union_iff in *.
+    destruct H1 as [Hc0_vs Hc0_vs0].
+    specialize (H4 _ Hc0_vs).
+    specialize (H2 _ Hc0_vs0).
+    apply ae_exp_sym in H4.
+    eapply ae_exp_trans;eauto.
+  + econstructor;eauto.
+Qed.
+
+Definition weakening Γ x τ σ (e : Exp) : Prop :=
+  x # Γ ->
+  [ Γ |- e ::: τ ] ->
+  [ Γ, x ::: σ |- e ::: τ ].
+
+Lemma weakening_α_compatible Γ x τ σ :
+  α_compatible (weakening Γ x τ σ).
+Proof.
+  intros e1 e2 Hα He1 Hx He2.
+  apply ae_exp_sym in Hα.
+  specialize (Typing_α_compatible Γ τ _ _ Hα) as H;cbn in *.
+  unfold weakening in *.
+  assert (Hwτ : [ Γ, x ::: σ |- e1 ::: τ]) by auto.
+  apply ae_exp_sym in Hα.
+  specialize (Typing_α_compatible (cons Γ x σ) τ _ _ Hα) as HH;cbn in *.
+  auto.
+Qed.
+
+Hint Constructors Typing_α.
+
+(* Lemma lookupEnv_fresh Γ x y τ: *)
+(*   x # Γ -> *)
+(*   lookEnv Γ  *)
+  
+
+Hint Resolve <- not_in_set_fresh.
+  
+
+Lemma weakening_Typing_α e Γ x:
+  (forall τ σ, weakening Γ x τ σ e).
+Proof.
+  (* apply Exp_alpha_equiv_ind. *)
+  (* apply Exp_alpha_equiv_ind. *)
+  apply (@Exp_alpha_equiv_ind_ctx (fun Γ x e => forall τ σ,  weakening Γ x τ σ e)).
+  + admit. (* apply weakening_α_compatible. *)
+  + intros ? ? ? ? ? ? Hty. inversion Hty;subst;auto.
+  + intros Γ0 ? a0 ? ? ? Hty. inversion Hty;subst.
+    assert (Ha : In a0 (supp Γ0)). admit.
+    assert (Hx: ~ In a (supp Γ0)) by eauto with set.
+    assert (a <> a0) by (apply not_eq_sym;eauto with set).
+    constructor.
+    cbn. now destruct (Atom.eq_dec a a0);tryfalse.
+  + intros Γ0 a. exists (singleton x).
+    (* exists (supp Γ). *)
+    intros a0 Hax e0 Hwe0 τ σ Hx Hty.
+    unfold weakening in *.
+    inversion Hty;subst;clear Hty.
+    assert (Ha_fresh : (a0 # (supp Γ0 : PFin) /\ a0 # (singleton x : PFin)) /\ a0 # (singleton a : PFin)) by now repeat rewrite <- fresh_union_iff.
+    eapply tyLam_α with (y:=a) (b1:=b1).
+    * apply fresh_cons_env;intuition;auto.
+    * apply ae_exp_refl.
+    * apply Hwe0.
+      ** apply fresh_cons_env;intuition;eauto with set.
+      ** eapply Typing_α_compatible.
+         inversion H3;subst.
+      unfold fresh;cbn. unfold AtomN.V.Disjoint. intuition;eauto with set.
+      unfold fresh. cbn.
+    rewrite Disjoint_spec.
+    intros ??.
+    rewrite SetProperties.P.add_union_singleton in *.
+    eauto with set.
+    
+    
+
